coq/Syntax.v
@@ -10,8 +10,11 @@ Section TrustformerSyntax.
 
     (* Given some variables, inputs and outputs we define our syntax *)
     Context {states_var: Type}.
+    Context {states_var_eqdec: EqDec states_var}.
     Context {inputs_var: Type}.
+    Context {inputs_var_eqdec: EqDec inputs_var}.
     Context {outputs_var: Type}.
+    Context {outputs_var_eqdec: EqDec outputs_var}.
 
     Inductive tf_unary_ops :=
         | tf_not                                (* Bitwise NOT *)
@@ -37,11 +40,13 @@ Section TrustformerSyntax.
         .
 
     Inductive tf_expr :=
-        | tf_const (value: nat)                                             (* Constant value *)
-        | tf_var (v: states_var)                                            (* Variable reference *) 
-        | tf_input (v: inputs_var)                                          (* Input reference *)
-        | tf_op1 (op: tf_unary_ops) (src: tf_expr)                          (* Unary operation *)
-        | tf_op2 (op: tf_binary_ops) (src1: tf_expr) (src2: tf_expr)        (* Binary operation *)
+        | tf_const (value: nat)                                                 (* Constant value *)
+        | tf_svar (v: states_var)                                               (* Variable reference *) 
+        | tf_ivar (v: inputs_var)                                               (* Input reference *)
+        | tf_ovar (v: outputs_var)                                              (* Output reference *)
+        | tf_op1 (op: tf_unary_ops) (src: tf_expr)                              (* Unary operation *)
+        | tf_op2 (op: tf_binary_ops) (src1: tf_expr) (src2: tf_expr)            (* Binary operation *)
+        | tf_expr_if (cond: tf_expr) (then_expr: tf_expr) (else_expr: tf_expr)  (* Conditional expression *)
         .
 
     (* Atomic operations on variables *)
@@ -56,6 +61,56 @@ Section TrustformerSyntax.
         | tf_ops_cons (op: tf_ops) (op2: tf_ops)                               (* Sequence of operations *)
         | tf_ops_if   (cond: tf_expr) (then_ops: tf_ops) (else_ops: tf_ops)    (* Conditional operations *)
         .
+        
+    Instance tf_unary_ops_eqdec: EqDec tf_unary_ops.
+    Proof.
+        constructor. intros.
+        decide equality.
+    Qed.
+
+    Instance tf_comparison_ops_eqdec: EqDec tf_comparison_ops.
+    Proof.
+        constructor. intros.
+        decide equality.
+    Qed.
+
+    Instance tf_binary_ops_eqdec: EqDec tf_binary_ops.
+    Proof.
+        constructor. intros.
+        decide equality;
+        try apply tf_comparison_ops_eqdec;
+        try apply Nat.eq_dec.
+    Qed.
+
+    Instance tf_expr_eqdec: EqDec tf_expr.
+    Proof.
+        constructor. intros.
+        decide equality;
+        try apply Nat.eq_dec;
+        try apply states_var_eqdec;
+        try apply inputs_var_eqdec;
+        try apply outputs_var_eqdec;
+        try apply tf_unary_ops_eqdec;
+        try apply tf_binary_ops_eqdec.
+    Qed.
+
+    Instance tf_op_eqdec: EqDec tf_op.
+    Proof.
+        constructor. intros.
+        decide equality;
+        try apply states_var_eqdec;
+        try apply outputs_var_eqdec;
+        try apply tf_expr_eqdec.
+    Qed.
+
+    Instance tf_ops_eqdec: EqDec tf_ops.
+    Proof.
+        constructor. intros.
+        decide equality;
+        try apply tf_op_eqdec;
+        try apply tf_expr_eqdec.
+    Qed.
+
 End TrustformerSyntax.
 
 (* Notations for Trustformer Syntax *)
@@ -63,9 +118,53 @@ End TrustformerSyntax.
     TODO: This is only temporary, to make some code more readable.
 *)
 
+Class IsExpr (S I O V : Type) := { 
+    as_expr : V -> @tf_expr S I O 
+}.
+
+Class IsAssignable (S I O V : Type) := { 
+    do_assign : V -> @tf_expr S I O -> @tf_op S I O 
+}.
+
+Class HasIf (Ret S I O : Type) := {
+    make_if : @tf_expr S I O -> Ret -> Ret -> Ret
+}.
+
+Arguments as_expr {S I O V} {_} _.
+Arguments do_assign {S I O V} {_} _ _.
+Arguments make_if {Ret S I O} {_} _ _ _.
+
+Instance StateIsExpr {S I O : Type} : IsExpr S I O S := {
+    as_expr := tf_svar
+}.
+
+Instance InputIsExpr {S I O : Type} : IsExpr S I O I := {
+    as_expr := tf_ivar
+}.
+
+Instance OutputIsExpr {S I O : Type} : IsExpr S I O O := {
+    as_expr := tf_ovar
+}.
+
+Instance StateIsAssignable {S I O : Type} : IsAssignable S I O S := {
+    do_assign := tf_assign
+}.  
+
+Instance OutputIsAssignable {S I O : Type} : IsAssignable S I O O := {
+    do_assign := tf_output
+}.
+
+Instance IfExpr {S I O : Type} : HasIf (@tf_expr S I O) S I O := {
+    make_if := tf_expr_if
+}.
+
+Instance IfOps {S I O : Type} : HasIf (@tf_ops S I O) S I O := {
+    make_if := tf_ops_if
+}.
+
 Declare Custom Entry trustformer.
-Declare Custom Entry tf_arg.   
-Declare Custom Entry tf_const.
+Declare Custom Entry tf_arg.     
+Declare Custom Entry tf_const.   
 
 Notation "{[ e ]}" := e (e custom trustformer at level 200).
 
@@ -73,14 +172,17 @@ Notation "x" := x (in custom tf_arg at level 0, x constr at level 0).
 Notation "n" := n (in custom tf_const at level 0, n constr at level 0).
 
 (* Variables & Constants *)
-Notation "'$S' x" := (tf_var x) 
-    (in custom trustformer at level 0, x custom tf_arg at level 0).
-
-Notation "'$I' x" := (tf_input x) 
-    (in custom trustformer at level 0, x custom tf_arg at level 0).
+Notation "'$' x" := (as_expr x) 
+    (in custom trustformer at level 0, x custom tf_arg at level 0, only parsing).
+Notation "'$' x" := (tf_svar x) 
+    (in custom trustformer at level 0, x custom tf_arg at level 0, format "'$' x", only printing).
+Notation "'$' x" := (tf_ivar x) 
+    (in custom trustformer at level 0, x custom tf_arg at level 0, format "'$' x", only printing).
+Notation "'$' x" := (tf_ovar x) 
+    (in custom trustformer at level 0, x custom tf_arg at level 0, format "'$' x", only printing).
 
 Notation "'#' n" := (tf_const n) 
-    (in custom trustformer at level 0, n custom tf_const at level 0).
+    (in custom trustformer at level 0, format "'#' n", n custom tf_const at level 0).
 
 (* Grouping *)
 Notation "'`' x '`'" := x (in custom trustformer at level 1, x constr at level 0).
@@ -100,36 +202,50 @@ Notation "x ^ y" := (tf_op2 tf_xor x y) (in custom trustformer at level 60, left
 
 (* Comparisons *)
 Notation "x <[ n ] y" := (tf_op2 (tf_cmp n tf_lt) x y) 
-    (in custom trustformer at level 70, n custom tf_const at level 0).
+    (in custom trustformer at level 70, n custom tf_const at level 0, format "x  <[ n ]  y").
 Notation "x <=[ n ] y" := (tf_op2 (tf_cmp n tf_le) x y) 
-    (in custom trustformer at level 70, n custom tf_const at level 0).
+    (in custom trustformer at level 70, n custom tf_const at level 0, format "x  <=[ n ]  y").
 Notation "x >[ n ] y" := (tf_op2 (tf_cmp n tf_gt) x y) 
-    (in custom trustformer at level 70, n custom tf_const at level 0).
+    (in custom trustformer at level 70, n custom tf_const at level 0, format "x  >[ n ]  y").
 Notation "x >=[ n ] y" := (tf_op2 (tf_cmp n tf_ge) x y) 
-    (in custom trustformer at level 70, n custom tf_const at level 0).
+    (in custom trustformer at level 70, n custom tf_const at level 0, format "x  >=[ n ]  y").
 Notation "x ==[ n ] y" := (tf_op2 (tf_cmp n tf_eq) x y) 
-    (in custom trustformer at level 70, n custom tf_const at level 0).
+    (in custom trustformer at level 70, n custom tf_const at level 0, format "x  ==[ n ]  y").
 Notation "x !=[ n ] y" := (tf_op2 (tf_cmp n tf_neq) x y) 
-    (in custom trustformer at level 70, n custom tf_const at level 0).
+    (in custom trustformer at level 70, n custom tf_const at level 0, format "x  !=[ n ]  y").
 
 (* Instructions *)
 Notation "'pass'" := (tf_ops_base tf_nop) (in custom trustformer at level 0).
 
-Notation "'let' '$S' x := e" := (tf_ops_base (tf_assign x e)) 
-    (in custom trustformer at level 80, x custom tf_arg at level 0).
-
-Notation "'let' '$O' x := e" := (tf_ops_base (tf_output x e)) 
-    (in custom trustformer at level 80, x custom tf_arg at level 0).
+Notation "'let' '$' x := e" := (tf_ops_base (do_assign x e))
+    (in custom trustformer at level 80, x custom tf_arg at level 0, only parsing).
+Notation "'let' '$' x := e" := (tf_ops_base (tf_assign x e)) 
+    (in custom trustformer at level 80, x custom tf_arg at level 0, format "'let'  $ x  :=  e", only printing).
+Notation "'let' '$' x := e" := (tf_ops_base (tf_output x e)) 
+    (in custom trustformer at level 80, x custom tf_arg at level 0, format "'let'  $ x  :=  e", only printing).
 
 Notation "s1 ; s2" := (tf_ops_cons s1 s2) 
     (in custom trustformer at level 90, right associativity, format "'[v' s1 ; '/' s2 ']'").
 
+Notation "'if' c 'then' t 'else' f" := (make_if c t f) 
+    (in custom trustformer at level 89, 
+    c custom trustformer at level 99, 
+    t custom trustformer at level 99, 
+    f custom trustformer at level 99,
+    only parsing).
 Notation "'if' c 'then' t 'else' f" := (tf_ops_if c t f) 
     (in custom trustformer at level 89, 
     c custom trustformer at level 99, 
     t custom trustformer at level 99, 
     f custom trustformer at level 99,
-    format "'[v' 'if'  c  'then' '/' t '/' 'else' '/' f ']'").
+    format "'[v' 'if'  c  'then' '/'   t '/' 'else' '/'   f ']'",
+    only printing).
+Notation "'if' c 'then' t 'else' f" := (tf_expr_if c t f) 
+    (in custom trustformer at level 89, 
+    c custom trustformer at level 99, 
+    t custom trustformer at level 99, 
+    f custom trustformer at level 99,
+    only printing).
 
 
 Section NotationExamples.
@@ -140,31 +256,48 @@ Section NotationExamples.
     Variables (s_a s_b : states_var) (i_x : inputs_var) (o_y : outputs_var).
 
     Definition t1 : @tf_ops states_var inputs_var outputs_var := {[ 
-        let $S s_a := $I i_x ;
-        let $S s_b := $I i_x
+        let $s_a := $i_x + #1;
+        let $s_b := $i_x
     ]}.
+    Goal True. pose (debug := t1); compute in debug.
+    Abort.
 
     Definition t2 : @tf_ops states_var inputs_var outputs_var := {[ 
-        if ($I i_x ==[32] $S s_a) 
-        then let $O o_y := #1 
-        else let $O o_y := #0
+        if ($i_x ==[32] $s_a) 
+        then 
+            let $o_y := #1;
+            pass 
+        else let $o_y := #0
     ]}.
+    Goal True. pose (debug := t2); compute in debug.
+    Abort.
 
     Definition t3 : @tf_ops states_var inputs_var outputs_var := {[ 
         pass ; pass                  
     ]}.
+    Goal True. pose (debug := t3); compute in debug.
+    Abort.
 
     Definition t4 : @tf_ops states_var inputs_var outputs_var := {[ 
-        let $S s_a := $I i_x + #1;                 
-        if ($S s_a ==[32] #10) 
-        then let $O o_y := $S s_a 
+        let $s_a := $i_x + #1;                 
+        if ($s_a ==[32] #10) 
+        then let $o_y := $s_a 
         else pass                           
     ]}.
-
+    Goal True. pose (debug := t4); compute in debug.
+    Abort.
 
     Definition t5 : @tf_ops states_var inputs_var outputs_var := {[ 
-        let $S s_a := $I (i_x) + `tf_const 1`;           
-        if ($S (s_a) ==[32] #10) then pass else pass
+        let $s_a := $i_x + `tf_const 1`;           
+        if ($s_a ==[32] #10) then pass else pass
     ]}.
+    Goal True. pose (debug := t5); compute in debug.
+    Abort.
+
+    Definition t6 : @tf_ops states_var inputs_var outputs_var := {[ 
+        let $s_a := if ($i_x ==[32] #0) then #1 else #2 
+    ]}.
+    Goal True. pose (debug := t6); compute in debug.
+    Abort.
 End NotationExamples.
 
