coq/Scheduler/VariableScheduler.v
@@ -1,0 +1,958 @@
+Require Import Koika.Frontend.
+Require Import Koika.Std.
+Require Import Koika.Utils.Common.
+Require Import Koika.Utils.Environments.
+Require Koika.BitsToLists.
+
+Require Import Coq.Logic.FunctionalExtensionality.
+
+Require Import Trustformer.Syntax.
+Require Import Trustformer.Semantics.
+Require Import Trustformer.Scheduler.Contract.
+Require Import Hammer.Plugin.Hammer.
+Set Hammer GSMode 63.
+
+Require Import Coq.Lists.List.
+Require Import Coq.Arith.Arith.
+Require Import Coq.Init.Nat.
+Require Import Coq.Program.Wf.
+
+Import ListNotations.
+
+Section SchedulerTypes.
+
+  Context {states_var: Type}.
+  Context {inputs_var: Type}.
+  Context {outputs_var: Type}.
+
+  Definition nid_t := nat.
+  Definition sz_t := nat.
+
+  Inductive dfg_vars_t := 
+    | DFG_SVar (v: states_var)
+    | DFG_OVar (v: outputs_var).
+
+  Inductive dfg_op_t :=
+    | DFG_Const (n: nat)
+    | DFG_Input (v: inputs_var)
+    | DFG_Var (v: dfg_vars_t)
+    | DFG_Unary (op: tf_unary_ops) (arg: nid_t)
+    | DFG_Binary (op: tf_binary_ops) (arg1: nid_t) (arg2: nid_t)
+    | DFG_Resize (arg: nid_t)
+    | DFG_Phi (cond: nid_t) (then_id: nid_t) (else_id: nid_t)
+    | DFG_Empty                
+    .
+
+  Record dfg_node_t := {
+    nid : nid_t;
+    op : dfg_op_t;
+    sz : sz_t;
+  }.
+
+  Record dfg_state_t := {
+    graph : list dfg_node_t;
+    var_map : list (dfg_vars_t * nid_t);
+  }.
+
+  Context {A} {buffer_needs: list (list A)}.
+
+  Inductive tf_dfg_states_t :=
+    | tf_dfg_done
+    | tf_dfg_s (state: states_var)
+    | tf_dfg_b (a_idx: Vect.index (length buffer_needs)) (n_idx: Vect.index (length (nth (index_to_nat a_idx) buffer_needs [])))
+    | tf_dfg_v (a_idx: Vect.index (length buffer_needs)) (n_idx: Vect.index (length (nth (index_to_nat a_idx) buffer_needs [])))
+    .
+        
+End SchedulerTypes.
+
+Section VariableScheduler.
+
+  Context (ctx: TFSchedContext).
+  Context (cost_limit: nat).
+
+  Local Notation states_var := (tfs_spec_states ctx).
+  Local Notation states_var_eq_dec := (tfs_spec_states_eq_dec ctx).
+  Local Notation states_var_fin := (tfs_spec_states_fin ctx).
+  Local Notation states_var_names := (tfs_spec_states_names ctx).
+  Local Notation states_var_size := (tfs_spec_states_size ctx).
+  Local Notation states_var_init := (tfs_spec_states_init ctx).
+
+  Local Notation inputs_var := (tfs_spec_inputs ctx).
+  Local Notation inputs_var_eq_dec := (tfs_spec_inputs_eq_dec ctx).
+  Local Notation inputs_var_fin := (tfs_spec_inputs_fin ctx).
+  Local Notation inputs_var_size := (tfs_spec_inputs_size ctx).
+
+  Local Notation outputs_var := (tfs_spec_outputs ctx).
+  Local Notation outputs_var_eq_dec := (tfs_spec_outputs_eq_dec ctx).
+  Local Notation outputs_var_fin := (tfs_spec_outputs_fin ctx).
+  Local Notation outputs_var_size := (tfs_spec_outputs_size ctx).
+
+  Local Notation spec_action := (tfs_spec_action ctx).
+  Local Notation spec_action_eq_dec := (tfs_spec_action_eq_dec ctx).
+  Local Notation spec_action_fin := (tfs_spec_action_fin ctx).
+  Local Notation spec_action_ops := (tfs_spec_action_ops ctx).
+  Local Notation spec_all_actions := (@finite_elements spec_action spec_action_fin).
+  Local Notation spec_action_index := (@finite_index spec_action spec_action_fin).
+
+  Hint Extern 0 (FiniteType states_var) => exact (tfs_spec_states_fin ctx) : typeclass_instances.
+  
+  Hint Extern 0 (Show states_var) => exact (tfs_spec_states_names ctx) : typeclass_instances.
+  Hint Extern 0 (Show inputs_var) => exact (tfs_spec_inputs_names ctx) : typeclass_instances.
+  Hint Extern 0 (Show outputs_var) => exact (tfs_spec_outputs_names ctx) : typeclass_instances.
+
+  (* ============================ *)
+  (* = Step 1: DFG Construction = *)
+  (* ============================ *)
+
+  (* --- DFG Definitions --- *)
+  Local Notation dfg_vars := (@dfg_vars_t states_var outputs_var).
+  Local Notation dfg_op := (@dfg_op_t states_var inputs_var outputs_var).
+  Local Notation dfg_node := (@dfg_node_t states_var inputs_var outputs_var).
+  Local Notation dfg_state := (@dfg_state_t states_var inputs_var outputs_var). 
+
+  Instance dfg_vars_eq_dec : EqDec dfg_vars.
+  Proof.
+    constructor. intros.
+    decide equality.
+    apply states_var_eq_dec.
+    apply outputs_var_eq_dec.
+  Defined.
+
+  Definition dfg_var_size (v: dfg_vars) : nat :=
+    match v with
+    | DFG_SVar sv => states_var_size sv
+    | DFG_OVar ov => outputs_var_size ov
+    end.
+
+  (* --- State Monad --- *)
+
+  Definition M (A : Type) := dfg_state -> (A * dfg_state).
+  Definition ret {A : Type} (x : A) : M A := fun s => (x, s).
+  Definition bind {A B : Type} (m : M A) (f : A -> M B) : M B :=
+    fun s => let (x, s') := m s in f x s'.
+  Notation "'let!' x ':=' m 'in' k" := (bind m (fun x => k)) (at level 60, right associativity).
+
+  Definition get_state : M dfg_state := fun s => (s, s).
+  Definition put_state (s : dfg_state) : M unit := fun _ => (tt, s).
+
+  (* --- Helpers --- *)
+
+  Definition emit (op : dfg_op) (sz: sz_t) : M nid_t :=
+    let! s := get_state in
+    let next_id := length (graph s) in
+    let new_node := {| nid := next_id; op := op; sz := sz |} in
+    let! _ := put_state ({| graph := new_node :: graph s; var_map := var_map s |}) in
+    ret next_id.
+
+  (* --- Variable & Output Management --- *)
+
+  Definition ensure_var (dfg_v: dfg_vars) : M nid_t :=
+    let! id := emit (DFG_Var dfg_v) (dfg_var_size dfg_v) in
+    let! s' := get_state in
+    let new_map := (dfg_v, id) :: filter (fun '(k, _) => if (eq_dec k dfg_v) then false else true) (var_map s') in
+    let! _ := put_state ({| graph := graph s'; var_map := new_map |}) in
+    ret id.
+
+  Definition get_var (dfg_v : dfg_vars) : M nid_t :=
+    let! s := get_state in
+      match BitsToLists.list_assoc (var_map s) dfg_v with
+      | Some id => ret id
+      | None => ensure_var dfg_v
+      end.
+
+  Definition set_var (dfg_v : dfg_vars) (id : nid_t) : M unit :=
+    let! s := get_state in
+    let new_map := (dfg_v, id) :: filter (fun '(k, _) => if (eq_dec k dfg_v) then false else true) (var_map s) in
+    put_state ({| graph := graph s; var_map := new_map |}).
+
+  (* --- Expression Compiler --- *)
+
+  Fixpoint dataflow_expr (e : tf_expr) (sz: sz_t) : M nid_t :=
+    match e with
+    | tf_const val => emit (DFG_Const val) sz
+    | tf_svar v => 
+      let! src_id := get_var (DFG_SVar v) in
+      if Nat.eqb (dfg_var_size (DFG_SVar v)) sz then
+        ret src_id
+      else
+        emit (DFG_Resize src_id) sz
+    | tf_ivar v => 
+      let! src_id := emit (DFG_Input v) sz in
+      if Nat.eqb (inputs_var_size v) sz then
+        ret src_id
+      else
+        emit (DFG_Resize src_id) sz
+    | tf_ovar v => 
+      let! src_id := get_var (DFG_OVar v) in
+      if Nat.eqb (dfg_var_size (DFG_OVar v)) sz then
+        ret src_id
+      else
+        emit (DFG_Resize src_id) sz
+    | tf_op1 op src =>
+      let! src_id := dataflow_expr src sz in
+      emit (DFG_Unary op src_id) sz
+    | tf_op2 op src1 src2 =>
+      match op with
+      | tf_cmp szC _ =>
+        let! id1 := dataflow_expr src1 szC in
+        let! id2 := dataflow_expr src2 szC in
+        emit (DFG_Binary op id1 id2) sz
+      | _ =>
+        let! id1 := dataflow_expr src1 sz in
+        let! id2 := dataflow_expr src2 sz in
+        emit (DFG_Binary op id1 id2) sz
+      end
+    | tf_expr_if cond then_expr else_expr =>
+      let! cond_id := dataflow_expr cond 1 in
+      let! then_id := dataflow_expr then_expr sz in
+      let! else_id := dataflow_expr else_expr sz in
+      emit (DFG_Phi cond_id then_id else_id) sz
+    end.
+
+  (* --- Generic Map Merger --- *)
+  
+  Definition merge_key 
+    (cond_id : nid_t) 
+    (k : dfg_vars) 
+    (val_t_opt val_e_opt : option nid_t) 
+    : M (option nid_t) :=
+    match val_t_opt, val_e_opt with
+    | Some vt, Some ve =>
+        if eq_dec vt ve then
+          ret (Some vt)
+        else 
+          let! phi := emit (DFG_Phi cond_id vt ve) (dfg_var_size k) in
+          ret (Some phi)
+    | Some vt, None => 
+        let! ve := ensure_var k in
+        let! phi := emit (DFG_Phi cond_id vt ve) (dfg_var_size k) in
+        ret (Some phi)
+    | None, Some ve =>
+        let! vt := ensure_var k in
+        let! phi := emit (DFG_Phi cond_id vt ve) (dfg_var_size k) in
+        ret (Some phi)
+    | None, None => ret None
+    end.
+
+  Fixpoint merge_loop 
+    (cond_id : nid_t)
+    (map_then map_else : list (dfg_vars * nid_t)) 
+    (keys : list (dfg_vars * nid_t)) 
+    (acc : list (dfg_vars * nid_t)) 
+    : M (list (dfg_vars * nid_t)) :=
+    match keys with
+    | [] => ret acc
+    | (k, _) :: rest =>
+        match BitsToLists.list_assoc acc k with
+        | Some _ => merge_loop cond_id map_then map_else rest acc
+        | None => 
+            let val_t := BitsToLists.list_assoc map_then k in
+            let val_e := BitsToLists.list_assoc map_else k in
+            
+            let! res_opt := merge_key cond_id k val_t val_e in
+            
+            match res_opt with
+            | Some final_id => merge_loop cond_id map_then map_else rest ((k, final_id) :: acc)
+            | None => merge_loop cond_id map_then map_else rest acc
+            end
+        end
+    end.
+
+  Definition merge_maps 
+    (cond_id : nid_t) 
+    (map_orig map_then map_else : list (dfg_vars * nid_t)) 
+    : M (list (dfg_vars * nid_t)) :=
+    
+    merge_loop cond_id map_then map_else (map_then ++ map_else) [].
+
+  (* --- Operations Compiler --- *)
+
+  Fixpoint dataflow_ops (ops : tf_ops) : M unit :=
+    match ops with
+    | tf_ops_base op =>
+      match op with
+      | tf_nop => ret tt
+      | tf_assign dst expr =>
+        let! res_id := dataflow_expr expr (dfg_var_size (DFG_SVar dst)) in
+        set_var (DFG_SVar dst) res_id
+      | tf_output dst expr =>
+        let! res_id := dataflow_expr expr (dfg_var_size (DFG_OVar dst)) in
+        set_var (DFG_OVar dst) res_id
+      end
+    | tf_ops_cons op1 op2 =>
+      let! _ := dataflow_ops op1 in
+      dataflow_ops op2
+    | tf_ops_if cond then_ops else_ops =>
+      let! cond_id := dataflow_expr cond 1 in
+      
+      let! s_orig := get_state in
+      
+      (* Then Branch *)
+      let! _ := dataflow_ops then_ops in
+      let! s_then := get_state in
+      
+      (* Restore maps *)
+      let! _ := put_state ({| 
+        graph := graph s_then; 
+        var_map := var_map s_orig
+      |}) in
+      
+      (* Else Branch *)
+      let! _ := dataflow_ops else_ops in
+      let! s_else := get_state in
+      
+      (* Merge Maps *)
+      let! final_vars := merge_maps cond_id 
+        (var_map s_orig) (var_map s_then) (var_map s_else) in
+    
+      (* Update final state *)
+      let! s := get_state in
+      put_state ({| 
+        graph := graph s; 
+        var_map := final_vars
+      |})
+    end.
+
+  (* --- Entry Point --- *)
+
+  Definition build_dfg (action : spec_action) : dfg_state :=
+    let ops := spec_action_ops action in
+    let empty_state := {| graph := [ {| nid := 0; op := DFG_Empty; sz := 0; |} ]; var_map := [] |} in
+    let (_, final_state) := dataflow_ops ops empty_state in
+    {| graph := rev (graph final_state); var_map := var_map final_state |}.
+
+  Definition get_args (node: dfg_node) : list nid_t :=
+    match op node with
+    | DFG_Const _ => []
+    | DFG_Input _ => []
+    | DFG_Var _ => []
+    | DFG_Unary _ arg => [arg]
+    | DFG_Binary _ arg1 arg2 => [arg1; arg2]
+    | DFG_Resize arg => [arg]
+    | DFG_Phi cond then_id else_id => [cond; then_id; else_id]
+    | DFG_Empty => []
+    end.
+
+  (* ============================ *)
+  (* = Step 2: Cost Calculation = *)
+  (* ============================ *)
+
+  Definition cost_t := nat.
+
+  Definition cost_fn (d: dfg_op) : cost_t :=
+    match d with
+    | DFG_Const _ => 0
+    | DFG_Input _ => 0
+    | DFG_Var _ => 0
+    | DFG_Unary op _ => match op with
+                      | tf_not => 1
+                      end
+    | DFG_Binary op _ _ => match op with
+                        | tf_and => 1
+                        | tf_or => 1
+                        | tf_xor => 1
+                        | tf_add => 2
+                        | tf_sub => 2
+                        | tf_mul => 5
+                        | tf_cmp _ _ => 1
+                        end
+    | DFG_Resize _ => 0
+    | DFG_Phi _ _ _ => 1
+    | DFG_Empty => 0
+    end.
+
+  Definition list_assoc_set_all_max {K: Type} {eq: EqDec K} (l: list (K * nat)) (k: list K) (v: nat)
+    : list (K * nat) :=
+    fold_left (fun acc key => 
+      if Nat.leb (match BitsToLists.list_assoc acc key with
+              | Some existing => existing
+              | None => 0
+              end) v then
+        BitsToLists.list_assoc_set acc key v
+      else
+        acc
+    ) k l.
+
+  Definition calc_backward_cost (dfg : dfg_state) : list (nid_t * cost_t) :=
+    let aux (cost_map: list (nid_t * cost_t)) (node : dfg_node) : list (nid_t * cost_t) :=
+      let cost := match BitsToLists.list_assoc cost_map (nid node) with
+                  | Some c => c
+                  | None => 0
+                  end in
+      list_assoc_set_all_max cost_map ((nid node) :: get_args node) (cost + cost_fn (op node))
+    in
+    fold_left aux (List.rev (graph dfg)) [].
+
+  (* 
+    Step 3, 4, 5, 6 are very simplistic for now.
+    Good performant HLS is not our focus, so we keep it simple.
+  *)
+
+  (* ============================== *)
+  (* = Step 3: Distance Splitting = *)
+  (* ============================== *)
+
+  Definition cycle_t := nat.
+
+  Definition calc_target_cycle (cost_map: list (nid_t * cost_t)) : list (nid_t * cycle_t) :=
+    map (fun '(nid, c) => (nid, c / cost_limit)) cost_map.
+
+  (* Definition calc_max_cycle (cost_map: list (nid_t * cycle_t)) : cycle_t :=
+    fold_left (fun amax '(_, c) => Nat.max amax c) cost_map 0. *)
+
+  (* ============================== *)
+  (* = Step 4: Buffer Allocation  = *)
+  (* ============================== *)
+
+  Definition require_buffer (dfg : dfg_state) (cycle_costs : list (nid_t * cycle_t)) : list (nid_t) :=
+    let aux (cost_map: list (nid_t)) (node : dfg_node) : list (nid_t) :=
+      let n_cycle := match BitsToLists.list_assoc cycle_costs (nid node) with
+                      | Some c => c
+                      | None => 0 (* should not happen *)
+                      end in
+      filter (fun x => match BitsToLists.list_assoc cycle_costs x with
+                      | Some c => negb (Nat.eqb c n_cycle)
+                      | None => false (* should not happen *)
+                      end ) (get_args node) ++ cost_map
+    in
+    nodup Nat.eq_dec (fold_left aux (graph dfg) []
+                        ++ filter (fun x => match BitsToLists.list_assoc cycle_costs x with
+                                          | Some 0 => false
+                                          | _ => true
+                                          end ) (map snd (var_map dfg))).
+
+  Definition get_sizes_and_idx (dfg : dfg_state) (nodes: list nid_t) : list (nid_t * (nat * sz_t)) :=
+    rev (fst (
+      fold_left (fun '(acc, idx) nid =>
+        let node := nth nid (graph dfg) {| nid := 0; op := DFG_Empty; sz := 0; |} in
+        ((nid, (idx, sz node)) :: acc, S idx)
+      ) nodes ([], 0))).
+
+  Definition buffer_needs 
+    :=
+    (* Determine the DFG of each operation *)
+    let dfgs := map build_dfg spec_all_actions in
+    (* Calculate the cost maps for each DFG *)
+    let cost_maps := map calc_backward_cost dfgs in
+    (* Calculate the target cycles for each node *)
+    let cycle_maps := map calc_target_cycle cost_maps in
+    (* Determine the required buffers across all actions *)
+    let buffers := map (fun '(dfg, cycle_map) => get_sizes_and_idx dfg (require_buffer dfg cycle_map)) (combine dfgs cycle_maps) in
+    
+    buffers.
+
+  Local Notation tf_dfg_states := (tf_dfg_states_t (states_var:=states_var) (buffer_needs:=buffer_needs)).
+  Definition test := tf_dfg_states.
+
+  Instance show_tf_dfg_states : Show tf_dfg_states :=
+    { show := fun dfg_s =>
+        match dfg_s with
+        | tf_dfg_s s => String.append "s_" (show s)
+        | tf_dfg_b a_idx n_idx => String.append "b_" (String.append (show (index_to_nat a_idx)) (String.append "_" (show (index_to_nat n_idx))))
+        | tf_dfg_v a_idx n_idx => String.append "v_" (String.append (show (index_to_nat a_idx)) (String.append "_" (show (index_to_nat n_idx))))
+        | tf_dfg_done => "done"
+        end }.
+
+  Definition tf_dfg_states_size (dfg_s: tf_dfg_states) : sz_t :=
+    match dfg_s with
+    | tf_dfg_s s => states_var_size s
+    | tf_dfg_b a_idx b_idx => snd (snd (nth (index_to_nat b_idx) (nth (index_to_nat a_idx) buffer_needs []) (0, (0, 0))))
+    | tf_dfg_v a_idx b_idx => 1
+    | tf_dfg_done => 1
+    end.
+
+  (* ============================== *)
+  (* = Step 5: Taint Analysis     = *)
+  (* ============================== *)
+
+  Definition get_tainted (dfg: dfg_state) : list (nid_t) :=
+    let aux (taint_map: list (nid_t)) (node : dfg_node) : list (nid_t) :=
+      let args := get_args node in
+      (* Secrets are tainted *)
+      let self_tainted := match op node with
+        | DFG_Var _ => true
+        | _ => false
+        end in
+      (* If node depends on secrets it is tainted *)
+      let is_tainted := self_tainted || existsb (fun arg_id =>
+        match mem arg_id taint_map with
+        | inl m => true
+        | inr _ => false
+        end) args 
+      in
+      (* If this node is output, then its no longer tainted *)
+      match mem (nid node) (map snd (var_map dfg)) with
+        | inl m => taint_map
+        | inr _ => if is_tainted then (nid node) :: taint_map else taint_map
+      end
+    in
+    fold_left aux (graph dfg) [].
+
+  (* ============================== *)
+  (* = Step 6: TF Compilations    = *)
+  (* ============================== *)
+
+  Local Notation expr_t := (@tf_expr tf_dfg_states inputs_var outputs_var).
+
+  Definition valid_expr_and (expr1: expr_t) (expr2: expr_t) : expr_t :=
+    match expr1, expr2 with
+    | tf_const 1, e2 => e2
+    | e1, tf_const 1 => e1
+    | _, _ => tf_op2 tf_and expr1 expr2
+    end.
+
+  Definition valid_expr_if (cond: expr_t) (then_expr: expr_t) (else_expr: expr_t) : expr_t :=
+    match then_expr, else_expr with
+    | tf_const 1, tf_const 1 => tf_const 1
+    | _, _ => tf_expr_if cond then_expr else_expr
+    end.
+
+  (* First the expression, then the valid signal *)
+  Fixpoint compile_dfg_expr (fuel: nat) (a_idx: Vect.index (length buffer_needs)) (dfg: dfg_state) (nid: nid_t) (buffers: list (nid_t * (nat * sz_t))) 
+    : (expr_t * expr_t)
+    :=
+    match fuel with
+    | 0 => (tf_const 0, tf_const 0) (* should not happen *)
+    | S fuel' =>
+        match BitsToLists.list_assoc buffers nid with
+        | Some (n_idx, n_sz) => match index_of_nat (length (nth (index_to_nat a_idx) buffer_needs [])) n_idx with
+                              | Some n_idx' => (tf_svar (tf_dfg_b a_idx n_idx'), tf_svar (tf_dfg_v a_idx n_idx'))
+                              | None => (tf_const 0, tf_const 0) (* should not happen *)
+                              end
+        | None => 
+          let node := nth nid (graph dfg) {| nid := 0; op := DFG_Empty; sz := 0; |} in
+          match op node with
+          | DFG_Const n => (tf_const n, tf_const 1)
+          | DFG_Input v => (tf_ivar v, tf_const 1)
+          | DFG_Var v => match v with
+                        | DFG_SVar s_var => (tf_svar (tf_dfg_s s_var), tf_const 1)
+                        | DFG_OVar o_var => (tf_ovar o_var, tf_const 1)
+                        end
+          | DFG_Unary op arg1 =>
+              let '(arg_expr, val_expr) := compile_dfg_expr fuel' a_idx dfg arg1 buffers in
+              (tf_op1 op arg_expr, val_expr)
+          | DFG_Binary op arg1 arg2 =>
+              let '(arg1_expr, val1_expr) := compile_dfg_expr fuel' a_idx dfg arg1 buffers in
+              let '(arg2_expr, val2_expr) := compile_dfg_expr fuel' a_idx dfg arg2 buffers in
+              (tf_op2 op arg1_expr arg2_expr, valid_expr_and val1_expr val2_expr)
+          | DFG_Resize arg1 =>
+              let '(arg_expr, val_expr) := compile_dfg_expr fuel' a_idx dfg arg1 buffers in
+              (arg_expr, val_expr)
+          | DFG_Phi cond_id then_id else_id =>
+              let '(cond_expr, cond_val) := compile_dfg_expr fuel' a_idx dfg cond_id buffers in
+              let '(then_expr, then_val) := compile_dfg_expr fuel' a_idx dfg then_id buffers in
+              let '(else_expr, else_val) := compile_dfg_expr fuel' a_idx dfg else_id buffers in
+              (
+                tf_expr_if cond_expr then_expr else_expr, 
+                if mem cond_id (get_tainted dfg) then
+                  valid_expr_and (valid_expr_and then_val else_val) cond_val
+                else
+                  valid_expr_and cond_val (valid_expr_if cond_expr then_val else_val)
+              )
+          | DFG_Empty => (tf_const 0, tf_const 0) (* should not happen *)
+          end
+        end
+    end.
+
+  Definition compile_dfg_buffers (a_idx: nat) (dfg: dfg_state) (buffers: list (nid_t * (nat * sz_t)))
+    := 
+    let fuel := length (graph dfg) in
+    match index_of_nat (length buffer_needs) a_idx with
+    | None => []
+    | Some a_idx' => 
+      flat_map 
+        ( fun '(nid, x) => 
+          match index_of_nat (length (nth (index_to_nat a_idx') buffer_needs [])) (fst x) with
+            | Some n_idx' => 
+              let buffers' := filter (fun '(b_nid, _) => negb (Nat.eqb b_nid nid)) buffers in
+              let '(expr, valid) := compile_dfg_expr fuel a_idx' dfg nid buffers' in
+              [ tf_assign (tf_dfg_b a_idx' n_idx') expr; tf_assign (tf_dfg_v a_idx' n_idx') valid ]
+            | None => [] (* should not happen *)
+            end ) buffers
+    end.
+
+  (* Fixpoint combine_pair_step (exprs : list expr_t) : list expr_t :=
+    match exprs with
+    | e1 :: e2 :: rest => (valid_expr_and e1 e2) :: combine_pair_step rest
+    | _ => exprs
+    end.
+
+  Fixpoint combine_balanced_helper (fuel : nat) (exprs : list expr_t) : expr_t :=
+    match fuel with
+    | 0 => tf_const 1 (* should not happen *)
+    | S f =>
+      match exprs with
+      | [] => tf_const 1
+      | [e] => e
+      | _ => combine_balanced_helper f (combine_pair_step exprs)
+      end
+    end.
+
+  Definition combine_valid_exprs (exprs : list expr_t) : expr_t :=
+    combine_balanced_helper (length exprs) exprs. *)
+
+  Fixpoint combine_valid_exprs (exprs: list (@tf_expr tf_dfg_states inputs_var outputs_var)) : @tf_expr tf_dfg_states inputs_var outputs_var :=
+    match exprs with
+    | [] => tf_const 1
+    | [e] => e
+    | e :: rest => valid_expr_and e (combine_valid_exprs rest)
+    end. 
+
+  Definition compile_dfg_aux (a_idx: nat) (dfg: dfg_state) (buffers: list (nid_t * (nat * sz_t))) :=
+    let fuel := length (graph dfg) in
+    match index_of_nat (length buffer_needs) a_idx with
+      | None => []
+      | Some a_idx' => 
+        map 
+          ( fun '(var, nid) => 
+            let '(expr, valid) := compile_dfg_expr fuel a_idx' dfg nid buffers in
+            match var with
+            | DFG_SVar sv =>
+              tf_assign (tf_dfg_s sv) expr
+            | DFG_OVar ov => 
+              tf_output ov expr
+            end
+            ) (var_map dfg)
+      end.
+
+  Definition compile_dfg_valid (a_idx: nat) (dfg: dfg_state) (buffers: list (nid_t * (nat * sz_t))) :=
+    let fuel := length (graph dfg) in
+    let nids := nodup Nat.eq_dec (map snd (var_map dfg)) in
+    let exprs := match index_of_nat (length buffer_needs) a_idx with
+      | None => []
+      | Some a_idx' => map ( fun nid => snd (compile_dfg_expr fuel a_idx' dfg nid buffers)) nids
+    end in
+    tf_assign tf_dfg_done (combine_valid_exprs exprs).
+
+  Definition schedule (act: spec_action)
+    (* : list (list (@tf_ops tf_dfg_states inputs_var outputs_var)) := *)
+    :=
+    let idx := spec_action_index act in
+    (* Determine the DFG of each operation *)
+    let dfgs := map build_dfg spec_all_actions in
+    (* Calculate the cost maps for each DFG *)
+    let cost_maps := map calc_backward_cost dfgs in
+    (* Calculate the target cycles for each node *)
+    let cycle_maps := map calc_target_cycle cost_maps in
+    (* Determine the required buffers across all actions *)
+    let buffers := map (fun '(dfg, cycle_map) => get_sizes_and_idx dfg (require_buffer dfg cycle_map)) (combine dfgs cycle_maps) in
+
+    let final_ops := compile_dfg_aux idx (nth idx dfgs {| graph := []; var_map := [] |}) (nth idx buffers []) in
+    let done_signal := compile_dfg_valid idx (nth idx dfgs {| graph := []; var_map := [] |}) (nth idx buffers []) in
+    
+    ( 
+      done_signal :: compile_dfg_buffers idx (nth idx dfgs {| graph := []; var_map := [] |}) (nth idx buffers []),
+      final_ops
+    ).
+
+  Definition done_signal := tf_dfg_done (states_var:=states_var) (buffer_needs:=buffer_needs).
+
+  Definition reset_states : list tf_dfg_states :=  
+    flat_map 
+      (fun a_idx => match index_of_nat (length buffer_needs) a_idx with
+        | Some a_idx' =>
+          flat_map (fun n_idx => match index_of_nat (length (nth (index_to_nat a_idx') buffer_needs [])) n_idx with
+            | Some n_idx' =>
+              [ tf_dfg_b a_idx' n_idx'; tf_dfg_v a_idx' n_idx' ]
+            | None => [] (* should not happen *)
+            end ) (List.seq 0 (length (nth (index_to_nat a_idx') buffer_needs [])))
+        | None => [] (* should not happen *)
+        end)
+      (List.seq 0 (length buffer_needs)).
+
+  Instance tf_dfg_states_fin2 : FiniteType2 tf_dfg_states.
+  Proof.  
+    unshelve econstructor.
+    - intro s. destruct s.
+      + exact (0, 0).
+      + exact (1, finite_index state).
+      + exact (2 + finite_index a_idx, finite_index n_idx).
+      + exact (2 + (Datatypes.length (finite_elements (T:=(Vect.index (Datatypes.length buffer_needs))))) + finite_index a_idx, finite_index n_idx).
+        
+    - refine ([ [tf_dfg_done] ] ++ 
+              [ map tf_dfg_s finite_elements ] ++ 
+              map (fun a => map (tf_dfg_b a) finite_elements) finite_elements ++ 
+              map (fun a => map (tf_dfg_v a) finite_elements) finite_elements).
+
+    - intros x n m EQ.
+      destruct x; inversion EQ; clear EQ; subst.
+      + (* tf_dfg_done *)
+        exists [tf_dfg_done]. split; auto.
+      + (* tf_dfg_s *)
+        exists (map tf_dfg_s finite_elements). split; auto.
+        rewrite map_nth_error with (d:=state); auto. rewrite finite_surjective. reflexivity.
+      + (* tf_dfg_b *)
+        exists (map (tf_dfg_b a_idx) finite_elements). split; auto.
+        * cbn [nth_error List.app].
+          apply nth_error_app_l.
+          rewrite map_nth_error with (d:=a_idx); auto.
+          change (index_to_nat a_idx) with (finite_index a_idx).
+          apply (finite_surjective a_idx).
+        * rewrite map_nth_error with (d:=n_idx); auto. 
+          change (index_to_nat n_idx) with (finite_index n_idx).
+          rewrite finite_surjective. reflexivity.
+      + (* tf_dfg_v *)
+        exists (map (tf_dfg_v a_idx) finite_elements). split.
+        * cbn [nth_error List.app].
+          rewrite nth_error_app2. 
+          2: {  repeat rewrite map_length. cbn. lia. }
+          repeat rewrite map_length. cbn.
+          rewrite Nat.add_comm, Nat.add_sub. 
+          rewrite map_nth_error with (d:=a_idx); auto.
+          change (index_to_nat a_idx) with (finite_index a_idx).
+          change (vect_to_list (all_indices (Datatypes.length buffer_needs))) with (finite_elements (T:=Vect.index (Datatypes.length buffer_needs))).
+          apply (finite_surjective a_idx).
+        * rewrite map_nth_error with (d:=n_idx); auto. 
+          change (index_to_nat n_idx) with (finite_index n_idx).
+          rewrite finite_surjective. reflexivity.
+    - intros n l Hn m x Hm.
+      destruct n as [|n].
+      { inversion Hn; subst. destruct m; inversion Hm; subst. reflexivity. timeout 10 scongruence use: nth_error_nil unfold: tfs_spec_states. }
+      destruct n as [|n].
+      { inversion Hn; subst. apply nth_error_map_inv in Hm. destruct Hm as [s [Hs ?]]; subst.
+        apply finite_elements_index in Hs. subst. reflexivity. }
+      
+      rewrite nth_error_app2 in Hn by (simpl; lia).
+      change (S (S n) - Datatypes.length [[tf_dfg_done]]) with (S n) in *.
+
+      cbn [nth_error List.app] in Hn.
+      destruct (lt_dec n (length (finite_elements (T := Vect.index (Datatypes.length buffer_needs))))) as [HLT | HGE].      
+      + rewrite nth_error_app1 in Hn by (rewrite map_length; auto).
+        apply nth_error_map_inv in Hn. destruct Hn as [a_idx' [Ha EQ_l]]; subst l.
+        apply nth_error_map_inv in Hm. destruct Hm as [n_idx' [Hn' EQ_x]]; subst x.
+
+        apply finite_elements_index in Ha.
+        apply finite_elements_index in Hn'.
+        subst n m. simpl. 
+        reflexivity.
+      + rewrite nth_error_app2 in Hn by (rewrite map_length; lia).
+        repeat rewrite map_length in Hn.
+        apply nth_error_map_inv in Hn. destruct Hn as [a_idx' [Ha EQ_l]]; subst l.
+        apply nth_error_map_inv in Hm. destruct Hm as [n_idx' [Hn' EQ_x]]; subst x.
+        apply finite_elements_index in Ha.
+        apply finite_elements_index in Hn'.
+        subst m. simpl. f_equal. 
+        (* hammer *) timeout 10 sauto.
+    - apply Forall_app; split; [| apply Forall_app; split].
+      + repeat constructor. (* hammer *) timeout 10 sfirstorder.
+      + repeat constructor. cbn [map]. rewrite map_map. apply NoDup_map_pair. apply finite_injective.
+      + apply Forall_app; split.
+        * (* Block for tf_dfg_b *)
+          apply Forall_map. apply Forall_forall. intros a_idx' Hin.
+          rewrite map_map. apply NoDup_map_pair.
+          apply finite_injective.
+        * (* Block for tf_dfg_v *)
+          apply Forall_map. apply Forall_forall. intros a_idx' Hin.
+          rewrite map_map. apply NoDup_map_pair.
+          apply finite_injective.
+  Defined.  
+
+  Instance tf_dfg_states_fin : FiniteType tf_dfg_states.
+  Proof.
+    apply FiniteType2_FiniteType.
+  Defined.
+
+  Definition maps_to (env: (ContextEnv (FT:=(tfs_spec_states_fin ctx))).(env_t) (tf_states_type states_var_size))
+    : ((ContextEnv (FT:=tf_dfg_states_fin)).(env_t) (tf_states_type tf_dfg_states_size)) :=
+    (ContextEnv (FT:=tf_dfg_states_fin)).(create) (
+      fun s =>
+        match s as s0 return (type_denote (tf_states_type tf_dfg_states_size s0)) with
+        | tf_dfg_s sv => getenv ContextEnv env sv
+        | tf_dfg_b a_idx n_idx => Bits.zero
+        | tf_dfg_v a_idx n_idx => Bits.zero
+        | tf_dfg_done => Bits.zero
+        end
+    ).
+
+  Definition maps_from (env: (ContextEnv (FT:=tf_dfg_states_fin)).(env_t) (tf_states_type tf_dfg_states_size))
+    : ((ContextEnv (FT:=(tfs_spec_states_fin ctx))).(env_t) (tf_states_type states_var_size)) :=
+    (ContextEnv (FT:=(tfs_spec_states_fin ctx))).(create) (
+      fun s =>
+        match s as s0 return (type_denote (tf_states_type states_var_size s0)) with
+        | sv => getenv ContextEnv env (tf_dfg_s sv)
+        end
+    ).
+
+  Definition tf_dfg_states_init (x: tf_dfg_states) : tf_states_type tf_dfg_states_size x :=
+    match x with
+    | tf_dfg_s sv => states_var_init sv
+    | tf_dfg_b _ _ => Bits.zero
+    | tf_dfg_v _ _ => Bits.zero
+    | tf_dfg_done => Bits.zero
+    end.
+
+  Definition tfs_schedule : TFSchedule :=
+    {|
+      tfs_ctx := ctx;
+
+      tfs_states := tf_dfg_states;
+      tfs_states_size := tf_dfg_states_size;
+      tfs_states_init := tf_dfg_states_init;
+      
+      tfs_inputs := inputs_var;
+      tfs_inputs_size := inputs_var_size;
+      tfs_inputs_fin := inputs_var_fin;
+
+      tfs_outputs := outputs_var;
+      tfs_outputs_size := outputs_var_size;
+      tfs_outputs_fin := outputs_var_fin;
+
+      tfs_action := spec_action;
+      tfs_action_fin := spec_action_fin;
+
+      tfs_map_to := maps_to;
+      tfs_map_from := maps_from;
+
+      tfs_schedule := schedule;
+      tfs_done_signal := done_signal;
+      tfs_reset_states := reset_states;
+    |}.
+
+End VariableScheduler.
+
+Module Examples.
+
+  Inductive dfge_s := x | y | z.
+  Definition dfge_s_size (s: dfge_s) : nat := 4.
+
+  Inductive dfge_i := in_A | in_B.
+  Definition dfge_i_size (i: dfge_i) : nat := 4.
+
+  Inductive dfge_o := out_A | out_B.
+  Definition dfge_o_size (o: dfge_o) : nat := 4.
+
+  Inductive dfge_a := action.
+
+  Definition shd_ctx1 : TFSchedContext :=
+    {|
+      tfs_spec_states := dfge_s;
+      tfs_spec_states_size := dfge_s_size;
+      tfs_spec_states_init := fun x => Bits.zero;
+
+      tfs_spec_inputs := dfge_i;
+      tfs_spec_inputs_size := dfge_i_size;
+
+      tfs_spec_outputs := dfge_o;
+      tfs_spec_outputs_size := dfge_o_size;
+
+      tfs_spec_action := dfge_a;
+      tfs_spec_action_ops := fun a =>
+        match a with
+        | _ => {[  
+            let $x := $in_A + #10;
+            let $out_A := $x + #1
+        ]}
+        end;
+    |}. 
+
+  Goal True. 
+    pose (cost := 10).
+    pose (shd := shd_ctx1).
+    pose (debug_dfg := build_dfg shd (action)); vm_compute in debug_dfg.
+    pose (debug_cost := calc_backward_cost shd debug_dfg); vm_compute in debug_cost.
+    pose (debug_cycle := calc_target_cycle cost debug_cost); vm_compute in debug_cycle.
+    pose (debug_bufs := require_buffer shd debug_dfg debug_cycle); vm_compute in debug_bufs.
+    pose (debug_sched := schedule shd cost (action)); vm_compute in debug_sched.
+  Abort.
+
+  Goal True. 
+    pose (cost := 4).
+    pose (shd := shd_ctx1).
+    pose (debug_dfg := build_dfg shd (action)); vm_compute in debug_dfg.
+    pose (debug_cost := calc_backward_cost shd debug_dfg); vm_compute in debug_cost.
+    pose (debug_cycle := calc_target_cycle cost debug_cost); vm_compute in debug_cycle.
+    pose (debug_bufs := require_buffer shd debug_dfg debug_cycle); vm_compute in debug_bufs.
+    pose (debug_sched := schedule shd cost (action)); time vm_compute in debug_sched. (* TIME: 0.2 Seconds *)
+  Abort.
+
+  Definition shd_ctx2 : TFSchedContext :=
+    {|
+      tfs_spec_states := dfge_s;
+      tfs_spec_states_size := dfge_s_size;
+      tfs_spec_states_init := fun x => Bits.zero;
+
+      tfs_spec_inputs := dfge_i;
+      tfs_spec_inputs_size := dfge_i_size;
+
+      tfs_spec_outputs := dfge_o;
+      tfs_spec_outputs_size := dfge_o_size;
+
+      tfs_spec_action := dfge_a;
+      tfs_spec_action_ops := fun a =>
+        match a with
+        | _ => {[  
+            let $x := $x * $x;
+            (if $in_A then
+              let $y := $x * $y + #1
+            else
+              pass
+            );
+            let $out_A := $y 
+        ]}
+        end;
+    |}.
+
+  Goal True. 
+    pose (cost := 15).
+    pose (shd := shd_ctx2).
+    pose (debug_dfg := build_dfg shd (action)); vm_compute in debug_dfg.
+    pose (debug_cost := calc_backward_cost shd debug_dfg); vm_compute in debug_cost.
+    pose (debug_cycle := calc_target_cycle cost debug_cost); vm_compute in debug_cycle.
+    pose (debug_bufs := require_buffer shd debug_dfg debug_cycle); vm_compute in debug_bufs.
+    pose (debug_sched := schedule shd cost (action)); vm_compute in debug_sched.
+  Abort.
+
+  Goal True. 
+    pose (cost := 5).
+    pose (shd := shd_ctx2).
+    pose (debug_dfg := build_dfg shd (action)); vm_compute in debug_dfg.
+    pose (debug_cost := calc_backward_cost shd debug_dfg); vm_compute in debug_cost.
+    pose (debug_cycle := calc_target_cycle cost debug_cost); vm_compute in debug_cycle.
+    pose (debug_bufs := require_buffer shd debug_dfg debug_cycle); vm_compute in debug_bufs.
+    pose (debug_sched := schedule shd cost (action)); time vm_compute in debug_sched.
+  Abort.
+
+  Definition no_precompute := schedule shd_ctx2 5 (action).
+  Definition with_precompute := tc_compute (schedule shd_ctx2 5 (action)).
+
+  Goal True.
+    pose (debug1 := no_precompute).
+    pose (debug2 := with_precompute).
+    time vm_compute in debug1.
+    time vm_compute in debug2.
+  Abort.
+
+  Definition shd_ctx3 : TFSchedContext :=
+    {|
+      tfs_spec_states := dfge_s;
+      tfs_spec_states_size := dfge_s_size;
+      tfs_spec_states_init := fun x => Bits.zero;
+
+      tfs_spec_inputs := dfge_i;
+      tfs_spec_inputs_size := dfge_i_size;
+
+      tfs_spec_outputs := dfge_o;
+      tfs_spec_outputs_size := dfge_o_size;
+
+      tfs_spec_action := dfge_a;
+      tfs_spec_action_ops := fun a =>
+        match a with
+        | _ => {[  
+            let $x := $y;
+            let $y := $z;
+            let $z := $x
+        ]}
+        end;
+    |}.
+
+  Goal True. 
+    pose (cost := 15).
+    pose (shd := shd_ctx3).
+    pose (debug_dfg := build_dfg shd (action)); vm_compute in debug_dfg.
+    pose (debug_cost := calc_backward_cost shd debug_dfg); vm_compute in debug_cost.
+    pose (debug_cycle := calc_target_cycle cost debug_cost); vm_compute in debug_cycle.
+    pose (debug_bufs := require_buffer shd debug_dfg debug_cycle); vm_compute in debug_bufs.
+    pose (debug_sched := schedule shd cost (action)); vm_compute in debug_sched.
+  Abort.
+
+End Examples.
